\documentclass{article}
\usepackage[margin=1in]{geometry}
\usepackage{amsmath}

\begin{document}

\section{Scalar operations}

\section{Vector operations}

\begin{enumerate}
\item Norm $\alpha = ||\mathbf{x}||_{2}$
\begin{itemize}
\item Forward: $\dot{\alpha} = \dfrac{ \mathbf{x}^{T} \dot{\mathbf{x}}}{||\mathbf{x}||_{2}}$
\item Reverse: $\bar{\mathbf{x}} = \dfrac{\bar{\alpha}}{||\mathbf{x}||_{2}} \mathbf{x}$
\end{itemize}

\item Scale $\mathbf{v} = \alpha \mathbf{x}$
\begin{itemize}
\item Forward: $\dot{\mathbf{v}} = \dot{\alpha} \mathbf{x} + \alpha \dot{\mathbf{x}}$
\item Reverse: $\bar{\alpha} = \bar{\mathbf{v}}^{T} \mathbf{x}$, $\bar{\mathbf{x}} = \alpha \bar{\mathbf{v}}$
\end{itemize}

\item AXPY $\mathbf{v} = \alpha \mathbf{x} + \mathbf{y}$
\begin{itemize}
\item Forward: $\dot{\mathbf{v}} = \dot{\alpha} \mathbf{x} + \alpha \dot{\mathbf{x}} + \dot{\mathbf{y}}$
\item Reverse: $\bar{\alpha} = \bar{\mathbf{v}}^{T} \mathbf{x}$, $\bar{\mathbf{x}} = \alpha \bar{\mathbf{v}}$, $\bar{\mathbf{y}} = \bar{\mathbf{v}}$
\end{itemize}

\item Dot-product $\alpha = \mathbf{x}^{T} \mathbf{y}$
\begin{itemize}
\item Forward: $\dot{\alpha} = \dot{\mathbf{x}}^{T} \mathbf{y} + \mathbf{x}^{T} \dot{\mathbf{y}}$
\item Reverse: $\bar{\mathbf{x}} = \bar{\alpha} \mathbf{y}$, $\bar{\mathbf{y}} = \bar{\alpha} \mathbf{x}$
\end{itemize}

\item Cross-product $\mathbf{v} = \mathbf{x} \times \mathbf{y}$,
\begin{itemize}
\item Forward: $\dot{\mathbf{v}} = \dot{\mathbf{x}} \times \mathbf{y} + \mathbf{x} \times \dot{\mathbf{y}}$
\item Reverse: $\bar{\mathbf{x}} = \mathbf{y} \times \bar{\mathbf{v}}$, $\bar{\mathbf{y}} = \bar{\mathbf{v}} \times \bar{\mathbf{x}}$,
\end{itemize}

\item Normalize $\mathbf{v} = \dfrac{\mathbf{x}}{||\mathbf{x}||_{2}}$
\begin{itemize}
\item Forward: $\dot{\mathbf{v}} = \dfrac{\dot{\mathbf{x}}}{||\mathbf{x}||_{2}} - \dfrac{(\dot{\mathbf{x}}^{T} \mathbf{x}) \mathbf{x}}{||\mathbf{x}||_{2}^{3}}$
\item Reverse: $\bar{\mathbf{x}} = \dfrac{\bar{\mathbf{v}}}{||\mathbf{x}||_{2}} - \dfrac{(\bar{\mathbf{v}}^{T} \mathbf{x}) \mathbf{x}}{||\mathbf{x}||_{2}^{3}}$
\end{itemize}

\item Symmetric outer-product $\mathbf{S} = \alpha \mathbf{x}\mathbf{x}^{T}$
\begin{itemize}
\item Forward: $\dot{\mathbf{S}} = \dot{\alpha}  \mathbf{x}\mathbf{x}^{T} + \alpha( \dot{\mathbf{x}} \mathbf{x}^{T} + \mathbf{x} \dot{\mathbf{x}}^{T})$
\item Reverse: $\bar{\alpha} = \mathbf{x}^{T} \bar{\mathbf{S}} \mathbf{x}$, $\bar{\mathbf{x}} = 2 \alpha \bar{\mathbf{S}} \mathbf{x}$
\end{itemize}

%\item Symmetric double outer-product $\mathbf{S} = \alpha (\mathbf{x} \mathbf{y}^{T} + \mathbf{y} \mathbf{x}^{T})$
%\begin{itemize}
%\item Forward: $\dot{\mathbf{S}} = \dot{\alpha}  (\mathbf{x} \mathbf{y}^{T} + \mathbf{y} \mathbf{x}^{T})$
%\end{itemize}

%\item Outer-product $\mathbf{A} = \alpha \mathbf{x}\mathbf{y}^{T}$
%\begin{itemize}
%\item Forward
%\item Reverse $\bar{\alpha} = \mathbf{x}^{T} \bar{\mathbf{A}} \mathbf{y}$, $\bar{x} = \alpha \bar{\mathbf{A}} \mathbf{y}$, $\bar{\mathbf{y}} = \alpha \bar{\mathbf{A}}^{T} \mathbf{x}$
%\end{itemize}

\end{enumerate}

\section{Matrix-vector operations}

\begin{enumerate}
\item Matrix-vector product $\mathbf{v} = \mathbf{A} \mathbf{x}$
\begin{itemize}
\item Forward: $\dot{\mathbf{v}} = \dot{\mathbf{A}} \mathbf{x} + \mathbf{A} \dot{\mathbf{x}}$
\item Reverse: $\bar{\mathbf{x}} = \mathbf{A}^{T} \bar{\mathbf{y}}$, $\bar{\mathbf{A}} = \bar{\mathbf{v}} \mathbf{x}^{T}$
\end{itemize}

\item Matrix-vector product $\mathbf{v} = \mathbf{A}^{T} \mathbf{x}$
\begin{itemize}
\item Forward: $\dot{\mathbf{v}} = \dot{\mathbf{A}}^{T} \mathbf{x} + \mathbf{A}^{T} \dot{\mathbf{x}}$
\item Reverse: $\bar{\mathbf{x}} = \mathbf{A} \bar{\mathbf{y}}$, $\bar{\mathbf{A}} = \mathbf{x} \bar{\mathbf{v}}^{T}$
\end{itemize}

% \item Inner product $\alpha = \mathbf{x}^{T} \mathbf{A} \mathbf{x}$
% \item Symmetric inner product $\alpha = \mathbf{x}^{T} \mathbf{S} \mathbf{x}$
\end{enumerate}

\section{Matrix-matrix operations}

\begin{enumerate}
\item Trace $\alpha = \text{tr}(\mathbf{A})$
\begin{itemize}
\item Forward $\dot{\alpha} = \text{tr}(\dot{\mathbf{A}})$
\item Reverse $\bar{\mathbf{A}}_{ii} = \bar{\alpha}$
\end{itemize}

\item Symmetric trace $\alpha = \text{tr}(\mathbf{S})$
\begin{itemize}
\item Forward $\dot{\alpha} = \text{tr}(\dot{\mathbf{S}})$
\item Reverse $\bar{\mathbf{S}}_{ii} = \bar{\alpha}$
\end{itemize}

\item Determinant $\alpha = \text{det}(\mathbf{A})$
\item Symmetric determinant $\alpha = \text{det}(\mathbf{A})$

\item Inverse $\mathbf{B} = \mathbf{A}^{-1}$
\begin{itemize}
\item Forward: $\dot{\mathbf{B}} = - \mathbf{A}^{-1} \dot{\mathbf{A}} \mathbf{A}^{-1}$
\item Reverse $\bar{\mathbf{A}} = - \mathbf{A}^{-T} \bar{\mathbf{B}} \mathbf{A}^{-T}$
\end{itemize}

\item Symmetric Inverse $\mathbf{T} = \mathbf{S}^{-1}$
\begin{itemize}
\item Forward: $\dot{\mathbf{T}} = - \mathbf{S}^{-1} \dot{\mathbf{S}} \mathbf{S}^{-1}$
\item Reverse $\bar{\mathbf{S}} = - \mathbf{S}^{-T} \bar{\mathbf{T}} \mathbf{S}^{-T}$
\end{itemize}

\item Symmetric part $\mathbf{S} = \alpha(\mathbf{A} + \mathbf{A}^{T})$
\item Anti-symmetric part $\mathbf{B} = \alpha (\mathbf{A} - \mathbf{A}^{T})$

\item Matrix addition $\mathbf{C} = \mathbf{A} + \mathbf{B}$
\begin{itemize}
\item Forward: $\dot{\mathbf{C}} =  \dot{\mathbf{A}} + \dot{\mathbf{B}}$
\item Reverse: $\bar{\mathbf{A}} =  \bar{\mathbf{C}}$, $\bar{\mathbf{B}} = \bar{\mathbf{C}}$
\end{itemize}

% tr(bar(C)^T dot(C)) = tr( B bar(C)^T dot(A)) + tr(bar(C)^{T} A dot(B))
% bar(B)^{T} = bar(C)^{T} A => bar(B) = A^{T} bar(C)
% bar(A)^{T} = B bar(C)^{T} => bar(A) = \bar{C} B^{T}

\item Matrix-matrix product $\mathbf{C} = \mathbf{A} \mathbf{B}$
\begin{itemize}
\item Forward $\dot{\mathbf{C}} = \dot{\mathbf{A}} \mathbf{B} + \mathbf{A} \dot{\mathbf{B}}$
\item Reverse $\bar{\mathbf{A}} = \bar{\mathbf{C}} \mathbf{B}^{T}$,  $\bar{\mathbf{B}} = \mathbf{A}^{T} \bar{\mathbf{C}}$,
\end{itemize}

\item Matrix-matrix product $\mathbf{C} = \mathbf{A}^{T} \mathbf{B}$
\begin{itemize}
\item Forward $\dot{\mathbf{C}} = \dot{\mathbf{A}}^{T} \mathbf{B} + \mathbf{A}^{T} \dot{\mathbf{B}}$
\item Reverse $\bar{\mathbf{A}} = \mathbf{B} \bar{\mathbf{C}}^{T}$,  $\bar{\mathbf{B}} = \mathbf{A} \bar{\mathbf{C}}$,
\end{itemize}

\item Matrix-matrix product $\mathbf{C} = \mathbf{A} \mathbf{B}^{T}$
\begin{itemize}
\item Forward $\dot{\mathbf{C}} = \dot{\mathbf{A}} \mathbf{B}^{T} + \mathbf{A} \dot{\mathbf{B}}^{T}$
\item Reverse $\bar{\mathbf{A}} = \bar{\mathbf{C}} \mathbf{B}$, $\bar{\mathbf{B}} = \bar{\mathbf{C}}^{T} \mathbf{A}$
\end{itemize}

\item Matrix-matrix product $\mathbf{C} = \mathbf{A}^{T} \mathbf{B}^{T}$
\begin{itemize}
\item Forward $\dot{\mathbf{C}} = \dot{\mathbf{A}}^{T} \mathbf{B}^{T} + \mathbf{A}^{T} \dot{\mathbf{B}}^{T}$
\item Reverse $\bar{\mathbf{A}} = \mathbf{B}^{T} \bar{\mathbf{C}}^{T} $, $\bar{\mathbf{B}} = \bar{\mathbf{C}}^{T} \mathbf{A}^{T}$
\end{itemize}

\item Linear Lagrange-Green strain $\mathbf{E} = \frac{1}{2} \left( \mathbf{U} + \mathbf{U}^{T} \right)$
\begin{itemize}
\item Forward $\dot{\mathbf{E}} = \frac{1}{2} \left( \dot{\mathbf{U}} + \dot{\mathbf{U}}^{T} \right)$
\item Reverse $\bar{\mathbf{U}} = \bar{\mathbf{E}}$
\end{itemize}

\item Lagrange-Green strain $\mathbf{E} = \frac{1}{2} \left( \mathbf{U} + \mathbf{U}^{T} + \mathbf{U}^{T} \mathbf{U} \right)$
\begin{itemize}
\item Forward $\dot{\mathbf{E}} = \frac{1}{2} \left( \dot{\mathbf{U}} + \dot{\mathbf{U}}^{T} + \dot{\mathbf{U}}^{T} \mathbf{U} + \mathbf{U}^{T} \dot{\mathbf{U}} \right)$
\item Reverse $\bar{\mathbf{U}} = (\mathbf{I} + \mathbf{U}) \bar{\mathbf{E}}$
\end{itemize}

\item Isotropic constitutive $\mathbf{S} = 2 \mu \mathbf{E} + \lambda \text{tr}(\mathbf{E}) \mathbf{I}$
\begin{itemize}
\item Forward $\dot{\mathbf{S}} = 2 \mu \dot{\mathbf{E}} + \lambda \text{tr}(\dot{\mathbf{E}}) \mathbf{I}$
\item Reverse $\bar{\mathbf{E}} = 2 \mu \bar{\mathbf{S}} + \lambda \text{tr}(\bar{\mathbf{S}}) \mathbf{I}$
\end{itemize}

\end{enumerate}

\end{document}
